{-# OPTIONS --without-K #-}

module Syntax where

{-
- Type syntax + substitution calculus
- Term syntax + substitution calculus
- Normal forms + renamings
-}

open import Lib

infixr 6 _∘'ₑ_
infixr 6 _ₑ∘'ₛ_ _ₛ∘'ₑ_ _∘'ₛ_
infixr 3 _⇒_
infix 3 _∈_


-- Type syntax
--------------------------------------------------------------------------------

data Con' : Set where
  ∙   : Con'
  _,* : Con' → Con'

data *∈ : Con' → Set where
  vz : ∀ {Δ} → *∈ (Δ ,*)
  vs : ∀ {Δ} → *∈ Δ → *∈ (Δ ,*)

data Ty (Δ : Con') : Set where
  var : *∈ Δ → Ty Δ
  _⇒_ : Ty Δ → Ty Δ → Ty Δ
  ∀'  : Ty (Δ ,*) → Ty Δ

-- Type embedding
--------------------------------------------------------------------------------

data OPE' : Con' → Con' → Set where
  ∙    : OPE' ∙ ∙
  drop : ∀ {Γ Δ} → OPE' Γ Δ → OPE' (Γ ,*) Δ
  keep : ∀ {Γ Δ} → OPE' Γ Δ → OPE' (Γ ,*) (Δ ,*)

id'ₑ : ∀ {Γ} → OPE' Γ Γ
id'ₑ {∙}    = ∙
id'ₑ {Γ ,*} = keep (id'ₑ {Γ})

wk' : ∀ {Γ} → OPE' (Γ ,*) Γ
wk' = drop id'ₑ

*∈ₑ : ∀ {Γ Δ} → OPE' Δ Γ → *∈ Γ → *∈ Δ
*∈ₑ ∙ ()
*∈ₑ (drop σ) v      = vs (*∈ₑ σ v)
*∈ₑ (keep σ) vz     = vz
*∈ₑ (keep σ) (vs v) = vs (*∈ₑ σ v)

Tyₑ : ∀ {Γ Δ} → OPE' Δ Γ → Ty Γ → Ty Δ
Tyₑ σ (var v) = var (*∈ₑ σ v)
Tyₑ σ (A ⇒ B) = Tyₑ σ A ⇒ Tyₑ σ B
Tyₑ σ (∀' A)  = ∀' (Tyₑ (keep σ) A)

_∘'ₑ_ : ∀ {Γ Δ Σ} → OPE' Δ Σ → OPE' Γ Δ → OPE' Γ Σ
σ      ∘'ₑ ∙      = σ
σ      ∘'ₑ drop δ = drop (σ ∘'ₑ δ)
drop σ ∘'ₑ keep δ = drop (σ ∘'ₑ δ)
keep σ ∘'ₑ keep δ = keep (σ ∘'ₑ δ)

ass'ₑ :
  ∀ {Γ Δ Σ Ξ}(σ : OPE' Σ Ξ)(δ : OPE' Δ Σ)(ν : OPE' Γ Δ)
  → (σ ∘'ₑ δ) ∘'ₑ ν ≡ σ ∘'ₑ (δ ∘'ₑ ν)
ass'ₑ σ        δ        ∙        = refl
ass'ₑ σ        δ        (drop ν) = drop & ass'ₑ σ δ ν
ass'ₑ σ        (drop δ) (keep ν) = drop & ass'ₑ σ δ ν
ass'ₑ (drop σ) (keep δ) (keep ν) = drop & ass'ₑ σ δ ν
ass'ₑ (keep σ) (keep δ) (keep ν) = keep & ass'ₑ σ δ ν

idr'ₑ : ∀ {Γ Δ}(σ : OPE' Γ Δ) → σ ∘'ₑ id'ₑ ≡ σ
idr'ₑ ∙        = refl
idr'ₑ (drop σ) = drop & idr'ₑ σ
idr'ₑ (keep σ) = keep & idr'ₑ σ

idl'ₑ : ∀ {Γ Δ}(σ : OPE' Γ Δ) → id'ₑ ∘'ₑ σ ≡ σ
idl'ₑ ∙        = refl
idl'ₑ (drop σ) = drop & idl'ₑ σ
idl'ₑ (keep σ) = keep & idl'ₑ σ

*∈-idₑ : ∀ {Γ}(v : *∈ Γ) → *∈ₑ id'ₑ v ≡ v
*∈-idₑ vz     = refl
*∈-idₑ (vs v) = vs & *∈-idₑ v

Ty-idₑ : ∀ {Γ}(A : Ty Γ) → Tyₑ id'ₑ A ≡ A
Ty-idₑ (var v) = var & *∈-idₑ v
Ty-idₑ (A ⇒ B) = _⇒_ & Ty-idₑ A ⊗ Ty-idₑ B
Ty-idₑ (∀' A)  = ∀' & Ty-idₑ A

*∈-∘ₑ : ∀ {Γ Δ Σ}(σ : OPE' Δ Σ)(δ : OPE' Γ Δ)(v : *∈ Σ) → *∈ₑ δ (*∈ₑ σ v) ≡ *∈ₑ (σ ∘'ₑ δ) v
*∈-∘ₑ ∙        ∙        ()
*∈-∘ₑ σ        (drop δ) v      = vs & *∈-∘ₑ σ δ v
*∈-∘ₑ (drop σ) (keep δ) v      = vs & *∈-∘ₑ σ δ v
*∈-∘ₑ (keep σ) (keep δ) vz     = refl
*∈-∘ₑ (keep σ) (keep δ) (vs v) = vs & *∈-∘ₑ σ δ v

Ty-∘ₑ : ∀ {Γ Δ Σ}(σ : OPE' Δ Σ)(δ : OPE' Γ Δ)(A : Ty Σ) → Tyₑ δ (Tyₑ σ A) ≡ Tyₑ (σ ∘'ₑ δ) A
Ty-∘ₑ σ δ (var v) = var & *∈-∘ₑ σ δ v
Ty-∘ₑ σ δ (A ⇒ B) = _⇒_ & Ty-∘ₑ σ δ A ⊗ Ty-∘ₑ σ δ B
Ty-∘ₑ σ δ (∀' A)  = ∀' & Ty-∘ₑ (keep σ) (keep δ) A

-- Type substitution
--------------------------------------------------------------------------------

data Sub' (Γ : Con') : Con' → Set where
  ∙   : Sub' Γ ∙
  _,_ : ∀ {Δ} → Sub' Γ Δ → Ty Γ → Sub' Γ (Δ ,*)

_ₛ∘'ₑ_ : ∀ {Γ Δ Σ} → Sub' Δ Σ → OPE' Γ Δ → Sub' Γ Σ
∙       ₛ∘'ₑ δ = ∙
(σ , A) ₛ∘'ₑ δ = (σ ₛ∘'ₑ δ) , Tyₑ δ A

_ₑ∘'ₛ_ : ∀ {Γ Δ Σ} → OPE' Δ Σ → Sub' Γ Δ → Sub' Γ Σ
∙      ₑ∘'ₛ δ       = δ
drop σ ₑ∘'ₛ (δ , A) = σ ₑ∘'ₛ δ
keep σ ₑ∘'ₛ (δ , A) = σ ₑ∘'ₛ δ , A

drop'ₛ : ∀ {Γ Δ} → Sub' Γ Δ → Sub' (Γ ,*) Δ
drop'ₛ σ = σ ₛ∘'ₑ wk'

keep'ₛ : ∀ {Γ Δ} → Sub' Γ Δ → Sub' (Γ ,*) (Δ ,*)
keep'ₛ σ = drop'ₛ σ , var vz

*∈ₛ : ∀ {Γ Δ} → Sub' Δ Γ → *∈ Γ → Ty Δ
*∈ₛ (σ , A) vz     = A
*∈ₛ (σ , _) (vs v) = *∈ₛ σ v

Tyₛ : ∀ {Γ Δ} → Sub' Δ Γ → Ty Γ → Ty Δ
Tyₛ σ (var v) = *∈ₛ σ v
Tyₛ σ (A ⇒ B) = Tyₛ σ A ⇒ Tyₛ σ B
Tyₛ σ (∀' A)  = ∀' (Tyₛ (keep'ₛ σ) A)

id'ₛ : ∀ {Γ} → Sub' Γ Γ
id'ₛ {∙}    = ∙
id'ₛ {Γ ,*} = keep'ₛ id'ₛ

ass'ₛₑₑ :
  ∀ {Γ Δ Σ Ξ}(σ : Sub' Σ Ξ)(δ : OPE' Δ Σ)(ν : OPE' Γ Δ)
  → (σ ₛ∘'ₑ δ) ₛ∘'ₑ ν ≡ σ ₛ∘'ₑ (δ ∘'ₑ ν)
ass'ₛₑₑ ∙       δ ν = refl
ass'ₛₑₑ (σ , A) δ ν = _,_ & ass'ₛₑₑ σ δ ν ⊗ Ty-∘ₑ δ ν A

ass'ₑₛₑ :
  ∀ {Γ Δ Σ Ξ}(σ : OPE' Σ Ξ)(δ : Sub' Δ Σ)(ν : OPE' Γ Δ)
  → (σ ₑ∘'ₛ δ) ₛ∘'ₑ ν ≡ σ ₑ∘'ₛ (δ ₛ∘'ₑ ν)
ass'ₑₛₑ ∙        δ       ν = refl
ass'ₑₛₑ (drop σ) (δ , A) ν = ass'ₑₛₑ σ δ ν
ass'ₑₛₑ (keep σ) (δ , A) ν = (_, Tyₑ ν A) & ass'ₑₛₑ σ δ ν

*∈-ₑ∘ₛ : ∀ {Γ Δ Σ}(σ : OPE' Δ Σ)(δ : Sub' Γ Δ)(v : *∈ Σ) → *∈ₛ δ (*∈ₑ σ v) ≡ *∈ₛ (σ ₑ∘'ₛ δ) v
*∈-ₑ∘ₛ ∙        δ       ()
*∈-ₑ∘ₛ (drop σ) (δ , A) v      = *∈-ₑ∘ₛ σ δ v
*∈-ₑ∘ₛ (keep σ) (δ , A) vz     = refl
*∈-ₑ∘ₛ (keep σ) (δ , A) (vs v) = *∈-ₑ∘ₛ σ δ v

Ty-ₑ∘ₛ :
  ∀ {Γ Δ Σ}(σ : OPE' Δ Σ)(δ : Sub' Γ Δ)(A : Ty Σ)
  → Tyₛ δ (Tyₑ σ A) ≡ Tyₛ (σ ₑ∘'ₛ δ) A
Ty-ₑ∘ₛ σ δ (var v) = *∈-ₑ∘ₛ σ δ v
Ty-ₑ∘ₛ σ δ (A ⇒ B) = _⇒_ & Ty-ₑ∘ₛ σ δ A ⊗ Ty-ₑ∘ₛ σ δ B
Ty-ₑ∘ₛ σ δ (∀' A)  = ∀' & (Ty-ₑ∘ₛ (keep σ) (keep'ₛ δ) A
                        ◾ (λ x → Tyₛ (x , var vz) A) & (ass'ₑₛₑ σ δ wk' ⁻¹))

*∈-ₛ∘ₑ : ∀ {Γ Δ Σ}(σ : Sub' Δ Σ)(δ : OPE' Γ Δ)(v : *∈ Σ) → Tyₑ δ (*∈ₛ σ v) ≡ *∈ₛ (σ ₛ∘'ₑ δ) v
*∈-ₛ∘ₑ (σ , A) δ vz     = refl
*∈-ₛ∘ₑ (σ , A) δ (vs v) = *∈-ₛ∘ₑ σ δ v

Ty-ₛ∘ₑ : ∀ {Γ Δ Σ}(σ : Sub' Δ Σ)(δ : OPE' Γ Δ)(A : Ty Σ) → Tyₑ δ (Tyₛ σ A) ≡ Tyₛ (σ ₛ∘'ₑ δ) A
Ty-ₛ∘ₑ σ δ (var v) = *∈-ₛ∘ₑ σ δ v
Ty-ₛ∘ₑ σ δ (A ⇒ B) = _⇒_ & Ty-ₛ∘ₑ σ δ A ⊗ Ty-ₛ∘ₑ σ δ B
Ty-ₛ∘ₑ σ δ (∀' A)  =
  ∀' & (Ty-ₛ∘ₑ (keep'ₛ σ) (keep δ) A
     ◾ (λ x → Tyₛ (x , var vz) A) &
         (ass'ₛₑₑ σ wk' (keep δ)
       ◾ (σ ₛ∘'ₑ_) & (drop & idl'ₑ δ)
       ◾ (σ ₛ∘'ₑ_) & (drop & (idr'ₑ δ ⁻¹))
       ◾ ass'ₛₑₑ σ δ wk' ⁻¹))

idr'ₛₑ : ∀ {Γ Δ}(σ : Sub' Δ Γ) → σ ₛ∘'ₑ id'ₑ ≡ σ
idr'ₛₑ ∙       = refl
idr'ₛₑ (σ , A) = _,_ & idr'ₛₑ σ ⊗ Ty-idₑ A

*∈-idₛ : ∀ {Γ}(v : *∈ Γ) → *∈ₛ id'ₛ v ≡ var v
*∈-idₛ vz     = refl
*∈-idₛ (vs v) = *∈-ₛ∘ₑ id'ₛ (drop id'ₑ) v ⁻¹
              ◾ Tyₑ (drop id'ₑ) & *∈-idₛ v
              ◾ var & (vs & *∈-idₑ v)

Ty-idₛ : ∀ {Γ} A → Tyₛ {Γ} id'ₛ A ≡ A
Ty-idₛ (var v) = *∈-idₛ v
Ty-idₛ (A ⇒ B) = _⇒_ & Ty-idₛ A ⊗ Ty-idₛ B
Ty-idₛ (∀' A)  = ∀' & Ty-idₛ A

emb'ₑ : ∀ {Γ Δ} → OPE' Γ Δ → Sub' Γ Δ
emb'ₑ ∙        = ∙
emb'ₑ (drop σ) = drop'ₛ (emb'ₑ σ)
emb'ₑ (keep σ) = keep'ₛ (emb'ₑ σ)

idr'ₑₛ : ∀ {Γ Δ}(σ : OPE' Γ Δ) → σ ₑ∘'ₛ id'ₛ ≡ emb'ₑ σ
idr'ₑₛ ∙        = refl
idr'ₑₛ (drop σ) = ass'ₑₛₑ σ id'ₛ wk' ⁻¹ ◾ (_ₛ∘'ₑ wk') & idr'ₑₛ σ
idr'ₑₛ (keep σ) = (_, var vz) & (ass'ₑₛₑ σ id'ₛ wk' ⁻¹ ◾ (_ₛ∘'ₑ wk') & idr'ₑₛ σ)

idl'ₛₑ : ∀ {Γ Δ}(σ : OPE' Γ Δ) → id'ₛ ₛ∘'ₑ σ ≡ emb'ₑ σ
idl'ₛₑ ∙        = refl
idl'ₛₑ (drop σ) =
    (λ x → id'ₛ ₛ∘'ₑ drop x) & (idr'ₑ σ ⁻¹)
  ◾ ass'ₛₑₑ id'ₛ σ wk' ⁻¹
  ◾ (_ₛ∘'ₑ wk') & idl'ₛₑ σ
idl'ₛₑ (keep σ) =
  (_, var vz) & (ass'ₛₑₑ id'ₛ wk' (keep σ)
  ◾ (λ x → id'ₛ ₛ∘'ₑ drop x) & (idl'ₑ σ ◾ idr'ₑ σ ⁻¹)
  ◾ ass'ₛₑₑ id'ₛ σ wk' ⁻¹
  ◾ (_ₛ∘'ₑ wk') & idl'ₛₑ σ)

_∘'ₛ_ : ∀ {Γ Δ Σ} → Sub' Δ Σ → Sub' Γ Δ → Sub' Γ Σ
∙       ∘'ₛ δ = ∙
(σ , A) ∘'ₛ δ = (σ ∘'ₛ δ) , Tyₛ δ A

ass'ₛₑₛ :
  ∀ {Γ Δ Σ Ξ}(σ : Sub' Σ Ξ)(δ : OPE' Δ Σ)(ν : Sub' Γ Δ)
  → (σ ₛ∘'ₑ δ) ∘'ₛ ν ≡ σ ∘'ₛ (δ ₑ∘'ₛ ν)
ass'ₛₑₛ ∙       δ ν = refl
ass'ₛₑₛ (σ , A) δ ν = _,_ & ass'ₛₑₛ σ δ ν ⊗ Ty-ₑ∘ₛ δ ν A

ass'ₛₛₑ :
  ∀ {Γ Δ Σ Ξ}(σ : Sub' Σ Ξ)(δ : Sub' Δ Σ)(ν : OPE' Γ Δ)
  → (σ ∘'ₛ δ) ₛ∘'ₑ ν ≡ σ ∘'ₛ (δ ₛ∘'ₑ ν)
ass'ₛₛₑ ∙       δ ν = refl
ass'ₛₛₑ (σ , A) δ ν = _,_ & ass'ₛₛₑ σ δ ν ⊗ Ty-ₛ∘ₑ δ ν A

idl'ₑₛ : ∀ {Γ Δ}(σ : Sub' Γ Δ) → id'ₑ ₑ∘'ₛ σ ≡ σ
idl'ₑₛ ∙       = refl
idl'ₑₛ (σ , A) = (_, A) & idl'ₑₛ σ

*∈-∘ₛ : ∀ {Γ Δ Σ}(σ : Sub' Δ Σ)(δ : Sub' Γ Δ) v → Tyₛ δ (*∈ₛ σ v) ≡ *∈ₛ (σ ∘'ₛ δ) v
*∈-∘ₛ (σ , A) δ vz     = refl
*∈-∘ₛ (σ , A) δ (vs v) = *∈-∘ₛ σ δ v

Ty-∘ₛ : ∀ {Γ Δ Σ}(σ : Sub' Δ Σ)(δ : Sub' Γ Δ) A → Tyₛ δ (Tyₛ σ A) ≡ Tyₛ (σ ∘'ₛ δ) A
Ty-∘ₛ σ δ (var v) = *∈-∘ₛ σ δ v
Ty-∘ₛ σ δ (A ⇒ B) = _⇒_ & Ty-∘ₛ σ δ A ⊗ Ty-∘ₛ σ δ B
Ty-∘ₛ σ δ (∀' A)  = ∀' & (Ty-∘ₛ (keep'ₛ σ) (keep'ₛ δ) A
                    ◾ (λ x → Tyₛ (x , var vz) A) & (ass'ₛₑₛ σ (drop id'ₑ) (keep'ₛ δ)
                    ◾ (σ ∘'ₛ_) & idl'ₑₛ (drop'ₛ δ)
                    ◾ ass'ₛₛₑ σ δ (drop id'ₑ) ⁻¹))

*∈-emb : ∀ {Γ Δ}(σ : OPE' Γ Δ) v → *∈ₛ (emb'ₑ σ) v ≡ var (*∈ₑ σ v)
*∈-emb ∙ ()
*∈-emb (drop σ) v =
    *∈-ₛ∘ₑ (emb'ₑ σ) (drop id'ₑ) v ⁻¹
  ◾ Tyₑ (drop id'ₑ) & *∈-emb σ v
  ◾ var & (vs & *∈-idₑ (*∈ₑ σ v))
*∈-emb (keep σ) vz     = refl
*∈-emb (keep σ) (vs v) =
    *∈-ₛ∘ₑ (emb'ₑ σ) (drop id'ₑ) v ⁻¹
  ◾ Tyₑ (drop id'ₑ) & *∈-emb σ v
  ◾ var & (vs & *∈-idₑ (*∈ₑ σ v))

Ty-emb : ∀ {Γ Δ}(σ : OPE' Γ Δ) A → Tyₛ (emb'ₑ σ) A ≡ Tyₑ σ A
Ty-emb σ (var v) = *∈-emb σ v
Ty-emb σ (A ⇒ B) = _⇒_ & Ty-emb σ A ⊗ Ty-emb σ B
Ty-emb σ (∀' A)  = ∀' & Ty-emb (keep σ) A

emb'-∘ₛ : ∀ {Γ Δ Σ}(σ : Sub' Δ Σ)(δ : OPE' Γ Δ) → σ ∘'ₛ emb'ₑ δ ≡ σ ₛ∘'ₑ δ
emb'-∘ₛ ∙       δ = refl
emb'-∘ₛ (σ , A) δ = _,_ & emb'-∘ₛ σ δ ⊗ Ty-emb δ A

-- Term syntax
--------------------------------------------------------------------------------

data Con : Con' → Set where
  ∙    : Con ∙
  _,_  : ∀ {Δ} → Con Δ → Ty Δ → Con Δ
  _,*  : ∀ {Δ} → Con Δ → Con (Δ ,*)

data _∈_ : ∀ {Δ} (A : Ty Δ) → Con Δ → Set where
  vz  : ∀ {Δ}{A : Ty Δ}{Γ}   → A ∈ (Γ , A)
  vs  : ∀ {Δ}{A : Ty Δ}{B Γ} → A ∈ Γ → A ∈ (Γ , B)
  vs* : ∀ {Δ}{A : Ty Δ}{Γ}   → A ∈ Γ → Tyₑ wk' A ∈ (Γ ,*)

data Tm {Δ} (Γ : Con Δ) : Ty Δ → Set where
  var  : ∀ {A} → A ∈ Γ → Tm Γ A
  lam  : ∀ {A B} → Tm (Γ , A) B → Tm Γ (A ⇒ B)
  app  : ∀ {A B} → Tm Γ (A ⇒ B) → Tm Γ A → Tm Γ B
  tlam : ∀ {A} → Tm (Γ ,*) A → Tm Γ (∀' A)
  tapp : ∀ {A} → Tm Γ (∀' A) → (B : Ty Δ) → Tm Γ (Tyₛ (id'ₛ , B) A)

-- Term embedding
--------------------------------------------------------------------------------

data OPE : ∀ {Γ Δ} → OPE' Γ Δ → Con Γ → Con Δ → Set where
  ∙     : OPE ∙ ∙ ∙
  drop' : ∀ {Γ Δ σ δ ν}   → OPE {Γ}{Δ} σ δ ν → OPE (drop σ) (δ ,*)         ν
  keep' : ∀ {Γ Δ σ δ ν}   → OPE {Γ}{Δ} σ δ ν → OPE (keep σ) (δ ,*)         (ν ,*)
  drop  : ∀ {Γ Δ σ δ ν A} → OPE {Γ}{Δ} σ δ ν → OPE σ        (δ , A)        ν
  keep  : ∀ {Γ Δ σ δ ν A} → OPE {Γ}{Δ} σ δ ν → OPE σ        (δ , Tyₑ σ A) (ν , A)

OPE'-of : ∀ {Γ' Δ' σ' Γ Δ} → OPE {Γ'}{Δ'} σ' Γ Δ → OPE' Γ' Δ'
OPE'-of {σ' = σ'} _ = σ'

Con'-of : ∀ {Γ} → Con Γ → Con'
Con'-of {Γ} _ = Γ

keepₜ : ∀ {Γ Δ σ δ ν A} → OPE {Γ}{Δ} σ δ ν → OPE σ (δ , Tyₑ σ A) (ν , A)
keepₜ = keep

idₑ : ∀ {Γ'}{Γ : Con Γ'} → OPE id'ₑ Γ Γ
idₑ {∙}     {∙}     = ∙
idₑ {∙}     {Γ , A} =
  coe ((λ x → OPE ∙ (Γ , x) (Γ , A)) & Ty-idₑ A) (keepₜ idₑ)
idₑ {Γ' ,*} {Γ , A} =
  coe ((λ x → OPE id'ₑ (Γ , x) (Γ , A)) & Ty-idₑ A) (keepₜ idₑ)
idₑ {Γ' ,*} {Γ ,*}  = keep' (idₑ {Γ'}{Γ})

∈ₑ : ∀ {Γ' Δ'}{σ' : OPE' Γ' Δ'}{Γ Δ A} →  OPE σ' Γ Δ → A ∈ Δ → Tyₑ σ' A ∈ Γ
∈ₑ ∙         ()
∈ₑ {A = A} (drop' {σ = σ} {δ} σ') v =
  coe
    ((_∈ (δ ,*)) & (Ty-∘ₑ σ wk' A ◾ (λ x → Tyₑ (drop x) A) & idr'ₑ σ))
  (vs* (∈ₑ σ' v))
∈ₑ (keep' {σ = σ} {δ} σ') (vs* {A = A} v) =
  coe
    ((_∈ (δ ,*)) & (Ty-∘ₑ σ wk' A
       ◾ (λ x → Tyₑ (drop x) A) & (idr'ₑ σ ◾ idl'ₑ σ ⁻¹) ◾ Ty-∘ₑ wk' (keep σ) A ⁻¹))
  (vs* (∈ₑ σ' v))
∈ₑ (drop σ)  v      = vs (∈ₑ σ v)
∈ₑ (keep σ) vz      = vz
∈ₑ (keep σ) (vs v)  = vs (∈ₑ σ v)

Tmₑ : ∀ {Γ' Δ'}{σ' : OPE' Γ' Δ'}{Γ Δ A} → OPE σ' Γ Δ → Tm Δ A → Tm Γ (Tyₑ σ' A)
Tmₑ σ (var v)    = var (∈ₑ σ v)
Tmₑ σ (lam t)    = lam (Tmₑ (keep σ) t)
Tmₑ σ (app f x)  = app (Tmₑ σ f) (Tmₑ σ x)
Tmₑ σ (tlam t)   = tlam (Tmₑ (keep' σ) t)
Tmₑ {σ' = σ'}{Γ} σ (tapp {A} t B) =
  coe (Tm Γ &
      (Ty-ₑ∘ₛ (keep σ') (id'ₛ , Tyₑ σ' B) A
    ◾ (λ x → Tyₛ (x , Tyₑ σ' B) A) &
        (idr'ₑₛ σ' ◾ idl'ₛₑ σ' ⁻¹) ◾ Ty-ₛ∘ₑ (id'ₛ , B) σ' A ⁻¹ ))
  (tapp (Tmₑ σ t) (Tyₑ σ' B))

_∘ₑ_ :
  ∀ {Γ' Δ' Σ' σ' δ' Γ Δ Σ} → OPE {Δ'}{Σ'} σ' Δ Σ → OPE {Γ'}{Δ'} δ' Γ Δ
  → OPE (σ' ∘'ₑ δ') Γ Σ
σ       ∘ₑ ∙       = σ
σ       ∘ₑ drop' δ = drop' (σ ∘ₑ δ)
σ       ∘ₑ drop  δ = drop  (σ ∘ₑ δ)
drop' σ ∘ₑ keep' δ = drop' (σ ∘ₑ δ)
keep' σ ∘ₑ keep' δ = keep' (σ ∘ₑ δ)
drop  σ ∘ₑ keep  δ = drop  (σ ∘ₑ δ)
_∘ₑ_ {σ' = σ'} {δ'} (keep {ν = ν} {A} σ) (keep {δ = δ₁} δ₂) =
  coe ((λ x → OPE (σ' ∘'ₑ δ') (δ₁ , x) (ν , A)) & (Ty-∘ₑ σ' δ' A ⁻¹))
  (keepₜ {A = A} (σ ∘ₑ δ₂))


-- options for proving things
-- 1. define and apply assloads of coe reduction rules (most tedious)
-- 2. define OTT-like structure for coercions (dunno how well it works)
-- 3. use proof automation, maybe throw in JMeq too (dunno how performant, how well it works
--                                                   in Agda)


-- Normal forms
--------------------------------------------------------------------------------

mutual
  data Nf {Γ} (Δ : Con Γ) : Ty Γ → Set where
    lam  : ∀ {A B} → Nf (Δ , A) B → Nf Δ (A ⇒ B)
    tlam : ∀ {A} → Nf (Δ ,*) A → Nf Δ (∀' A)
    ne   : ∀ {v} → Ne Δ (var v) → Nf Δ (var v)

  data Ne {Γ}(Δ : Con Γ) : Ty Γ → Set where
    var  : ∀ {A} → A ∈ Δ → Ne Δ A
    app  : ∀ {A B} → Ne Δ (A ⇒ B) → Nf Δ A → Ne Δ B
    tapp : ∀ {A} → Ne Δ (∀' A) → (B : Ty Γ) → Ne Δ (Tyₛ (id'ₛ , B) A)

tappₙₑ : ∀ {Γ}{Δ : Con Γ}{A} → Ne Δ (∀' A) → (B : Ty Γ) → Ne Δ (Tyₛ (id'ₛ , B) A)
tappₙₑ = tapp

mutual
  Nfₑ : ∀ {Γ' Γ Δ' Δ σ' A} → OPE {Γ'}{Δ'} σ' Γ Δ → Nf Δ A → Nf Γ (Tyₑ σ' A)
  Nfₑ σ (lam t)  = lam (Nfₑ (keep σ) t)
  Nfₑ σ (tlam t) = tlam (Nfₑ (keep' σ) t)
  Nfₑ σ (ne n)   = ne (Neₑ σ n)

  Neₑ : ∀ {Γ' Γ Δ' Δ A σ'} → OPE {Γ'}{Δ'} σ' Γ Δ → Ne Δ A → Ne Γ (Tyₑ σ' A)
  Neₑ σ (var v)    = var (∈ₑ σ v)
  Neₑ σ (app n t)  = app (Neₑ σ n) (Nfₑ σ t)
  Neₑ {Γ = Γ}{σ' = σ'} σ (tapp {A} n B) =
    coe (Ne Γ &
         (Ty-ₑ∘ₛ (keep σ') (id'ₛ , Tyₑ σ' B) A
       ◾ (λ x → Tyₛ (x , Tyₑ σ' B) A) & (idr'ₑₛ σ' ◾ idl'ₛₑ σ' ⁻¹)
       ◾ Ty-ₛ∘ₑ (id'ₛ , B) σ' A ⁻¹))
    (tappₙₑ (Neₑ σ n) (Tyₑ (OPE'-of σ) B))

-- Term substitution
---------------------------------------------------------------------------------

